Everything seems to compile.  Had a strange error previously, not quite sure why.

binheap/verif_binary_heap.v
@@ -132,8 +132,8 @@ Definition build_heap_spec :=
     LOCAL ()
     SEP (harray arr_contents' arr).
 
-Definition heapsort_spec :=
-  DECLARE _heap_sort WITH arr : val, arr_contents : list heap_item, size : Z
+Definition heapsort_rev_spec :=
+  DECLARE _heapsort_rev WITH arr : val, arr_contents : list heap_item, size : Z
   PRE [tptr t_item, tuint]
     PROP (size > 0 ;
           Zlength arr_contents = size)
@@ -151,9 +151,9 @@ Definition Gprog : funspecs :=
          ltac:(with_library prog [ exch_spec ; less_spec ; swim_spec ; sink_spec ; 
                                    remove_min_nc_spec ; insert_nc_spec ; 
                                    size_spec ; capacity_spec ; 
-                                   build_heap_spec ; heapsort_spec ]).
+                                   build_heap_spec ; heapsort_rev_spec ]).
 
-Lemma body_heapsort: semax_body Vprog Gprog f_heap_sort heapsort_spec.
+Lemma body_heapsort: semax_body Vprog Gprog f_heapsort_rev heapsort_rev_spec.
 Proof.
   start_function.
   assert_PROP (2 * (size - 2) <= Int.max_unsigned). { 
@@ -164,7 +164,8 @@ Proof.
   Intros arr_contents'.
   forward.
   forward_loop (EX s : Z, EX arr_contents1 : list heap_item, EX arr_contents2 : list heap_item,
-                 PROP (s = Zlength arr_contents1;
+                 PROP (s > 0 ;
+                       s = Zlength arr_contents1;
                        heap_ordered arr_contents1;
                        Sorted (Basics.flip cmp_rel) arr_contents2;
                        Forall (fun x => HdRel (Basics.flip cmp_rel) x arr_contents2) arr_contents1;
@@ -175,21 +176,26 @@ Proof.
     rewrite app_nil_r. entailer!. split. apply Permutation_Zlength. trivial.
     apply Forall_forall. constructor. }
   Intros s arrc1 arrc2.
-  generalize (Permutation_Zlength _ _ _ H8); intro.
-  rewrite Zlength_app in H9.
+  generalize (Permutation_Zlength _ _ _ H9); intro.
+  rewrite Zlength_app in H10.
   forward_if.
-  2: { assert (s = 0) by rep_lia. subst s. destruct arrc1.
-    2: rewrite Zlength_cons in H11; rep_lia.
-    rewrite app_nil_l in *. rewrite H11, Z.add_0_l in *. 
-    forward. Exists arrc2. entailer!. }
+  2: { assert (s = 1) by rep_lia. subst s.
+       destruct arrc1. rewrite Zlength_nil in H12; lia.
+       destruct arrc1. 2: do 2 rewrite Zlength_cons in H12; rep_lia.
+       rewrite H12.
+       forward. Exists (h :: arrc2). entailer!. 2: apply derives_refl.
+       constructor. trivial. rewrite Forall_forall in H8.
+       apply H8. left. trivial. }
   forward.
   rewrite harray_split. Intros.
   forward_call (0, s-1, arr, arrc1). rep_lia.
-  destruct arrc1. rewrite Zlength_nil in H4. lia.
+  destruct arrc1. rewrite Zlength_nil in H5. lia.
   generalize (foot_split_spec _ (h :: arrc1)). case foot_split. destruct o. 2: intros [? ?]; subst; discriminate.
-  intros. destruct l. destruct arrc1. 2: discriminate. inversion H11. subst h0. clear H11.
-  { (* Degenerate case: only one item! *)
-    rewrite Zlength_one in H4. subst s. simpl.
+  intros. destruct l. destruct arrc1. 2: discriminate. inversion H12. subst h0. clear H12.
+  { (* Degenerate case: only one item, which simplies nicely after chaning the bound! *)
+    rewrite Zlength_one in H5. lia. }
+
+(*  subst s. simpl.
     rewrite Zexchange_eq.
     rewrite Int.sub_idem.
     change [h] with (nil ++ [h]) at 1.
@@ -206,10 +212,11 @@ Proof.
     Exists 0 (@nil heap_item) (h :: arrc2). entailer!.
     split. apply heapOrdered_empty. constructor. trivial. inversion H7. trivial.
     rewrite <- harray_split. simpl. change (h :: arrc2) with ([h] ++ arrc2).
-    rewrite <- harray_split. apply derives_refl. }
+    rewrite <- harray_split. apply derives_refl. } *)
+
   (* Main line *)
-  assert (h1 = h) by (inversion H11; auto). subst h1.
-  rewrite H11 in *. clear H11 arrc1.
+  assert (h1 = h) by (inversion H12; auto). subst h1.
+  rewrite H12 in *. clear H12 arrc1.
   replace (s - 1) with (Zlength (h :: l)).
   2: autorewrite with sublist in *; rep_lia.
   rewrite Zexchange_head_foot.
@@ -219,29 +226,29 @@ Proof.
     split. rep_lia. split. intros _. rep_lia.
     apply weak_heapOrdered_bounded_root_weak_heapOrdered.
     eapply weak_heapOrdered_root.
-    apply heapOrdered_cutfoot in H5. apply H5. }
+    apply heapOrdered_cutfoot in H6. apply H6. }
   Intros arrc1. Exists (s-1) arrc1 (h :: arrc2). entailer!.
-  { split. apply Permutation_Zlength in H12. autorewrite with sublist in *. trivial.
-    split. apply heapOrdered_bounded_root_heapOrdered. apply H11.
-    split. constructor. trivial. inversion H7. trivial.
+  { split. apply Permutation_Zlength in H13. autorewrite with sublist in *. trivial.
+    split. apply heapOrdered_bounded_root_heapOrdered. apply H12.
+    split. constructor. trivial. inversion H8. trivial.
     split.
     * apply Forall_forall. intros. constructor.
-      symmetry in H12.
-      generalize (Permutation_in x H12 H0); intro.
-      generalize (root_minimal _ cmp_rel cmp_po _ H5 h eq_refl); intro.
-      rewrite Forall_forall in H13. apply H13.
+      symmetry in H13.
+      generalize (Permutation_in x H13 H0); intro.
+      generalize (root_minimal _ cmp_rel cmp_po _ H6 h eq_refl); intro.
+      rewrite Forall_forall in H14. apply H14.
       rewrite <- app_comm_cons. right.
       apply in_or_app.
-      destruct H4. subst x. right. left. trivial. auto.
+      destruct H5. subst x. right. left. trivial. auto.
     * apply Permutation_trans with (((h :: l) ++ [h0]) ++ arrc2). trivial.
       change (h :: arrc2) with ([h] ++ arrc2). rewrite app_assoc.
       apply Permutation_app. 2: apply Permutation_refl.
       apply Permutation_trans with (h :: arrc1).
       2: apply Permutation_cons_append.
       simpl. constructor.
-      apply Permutation_app_comm_trans. apply H12. }
-  { apply Permutation_Zlength in H12.
-    rewrite Zlength_app. rewrite H12. rewrite <- Zlength_app.
+      apply Permutation_app_comm_trans. apply H13. }
+  { apply Permutation_Zlength in H13.
+    rewrite Zlength_app. rewrite H13. rewrite <- Zlength_app.
     rewrite <- harray_split.
     rewrite Zlength_app.
     replace (Zlength ((h :: l) ++ [h0])) with (Zlength (arrc1 ++ [h])).
@@ -600,16 +607,15 @@ Proof.
     inversion H. subst foot. clear H Hx.
     simpl.
     forward_call (0, arr, @nil heap_item, 0, 0); rewrite Zlength_nil. 
-      { unfold harray. rewrite data_at_isptr. entailer. (* Surely there's a less heavy hammer way to do this? *)
+      { rewrite Zexchange_eq. unfold harray. rewrite data_at_isptr. entailer. (* Surely there's a less heavy hammer way to do this? *)
         rewrite data_at_zero_array_eq; auto. entailer!. }
       { split; auto. split; auto. split. rep_lia. split. rep_lia.
         apply weak_heapOrdered_bounded_root_weak_heapOrdered.
         apply hOwhO. apply cmp_po. apply heapOrdered_empty. }
     (* Prove postcondition *)
     Intro vret. Exists (n, vret) root. entailer. (* Surely there's a less heavy hammer way to do this? *)
-    destruct H. apply Permutation_nil in H13. subst vret. clear H Hy.
+    apply Permutation_nil in H3. subst vret. clear H Hy.
     sep_apply harray_emp. rewrite emp_sepcon.
-    rewrite Zlength_Zexchange. rewrite Zexchange_eq.
     do 2 rewrite fold_harray. unfold valid_pq, hitem.
     apply andp_right. apply prop_right. auto.
     Exists arr (root :: junk). simpl. entailer!.
@@ -633,22 +639,21 @@ Proof.
     (* Prove postcondition *)
     Intro vret. Exists (n, vret) root. simpl fst. unfold hitem, heap_item_rep, heap_size, heap_capacity. simpl fst. simpl snd. entailer!.
       { (* Pure part *)
-        split. constructor. rewrite H5. transitivity ([foot] ++ l0). apply Permutation_app_comm. destruct H4. auto.
+        split. constructor. rewrite H5. transitivity ([foot] ++ l0). apply Permutation_app_comm. auto.
         generalize (root_minimal _ _ _ _ H1 root eq_refl); intro.
-        rewrite H5 in H10. apply Forall_inv_tail in H10.
-        eapply forall_permutation. apply H10. transitivity ([foot] ++ l0). apply Permutation_app_comm. simpl. tauto. }
+        rewrite H5 in H11. apply Forall_inv_tail in H11.
+        eapply forall_permutation. apply H11. transitivity ([foot] ++ l0). apply Permutation_app_comm. simpl. tauto. }
     unfold valid_pq. Exists arr (root :: junk). unfold heap_size, heap_capacity. simpl.
-    destruct H4.
-    replace (Zlength vret) with (Zlength (root :: l0)). 2: { apply Permutation_Zlength in H10. trivial. }
+    replace (Zlength vret) with (Zlength (root :: l0)). 2: { apply Permutation_Zlength in H6. trivial. }
     apply heapOrdered_bounded_root_heapOrdered in H4.
     entailer!. { (* Pure part inside spatial part *)
-      simpl fst in H2. rewrite <- H2. apply Permutation_Zlength in H10. autorewrite with sublist. rewrite <- H10.
+      simpl fst in H2. rewrite <- H2. apply Permutation_Zlength in H6. autorewrite with sublist. rewrite <- H6.
       simpl snd. autorewrite with sublist in *. lia. }
     (* Spatial part, this seems a bit uglier than necessary? *)
     change (root :: junk) with ([root] ++ junk). rewrite app_assoc. do 2 rewrite harray_split.
-    apply Permutation_Zlength in H10.
-    rewrite app_comm_cons. rewrite Zlength_app. rewrite H10. rewrite Zlength_app.
-    assert (Zlength (root :: l0) = Zlength vret). { rewrite <- H10. do 2 rewrite Zlength_cons. trivial. }
+    apply Permutation_Zlength in H6.
+    rewrite app_comm_cons. rewrite Zlength_app. rewrite H6. rewrite Zlength_app.
+    assert (Zlength (root :: l0) = Zlength vret). { rewrite <- H6. do 2 rewrite Zlength_cons. trivial. }
     do 3 rewrite app_comm_cons.
     do 4 rewrite Zlength_app. rewrite H11.
     do 2 rewrite Zlength_one.
